Definition of target lang, and WIP back-translation from STLC to it

state/TargetLang.fst
@@ -6,331 +6,54 @@ open FStar.Tactics.Typeclasses
 open SharedRefs
 open Witnessable
 
-open STLC
+type targetlang_pspec = 
+  (inv:heap -> Type0) * (prref:ref_pred) * (hrel:FStar.Preorder.preorder heap)
 
-let rec to_shareable_typ (t:typ0) : shareable_typ =
-  match t with
-  | TUnit -> SUnit
-  | TNat -> SNat
-  | TSum t1 t2 -> SSum (to_shareable_typ t1) (to_shareable_typ t2)
-  | TPair t1 t2 -> SPair (to_shareable_typ t1) (to_shareable_typ t2)
-  | TRef t -> SRef (to_shareable_typ t)
-  | TLList t -> SLList (to_shareable_typ t)
+class targetlang (spec:targetlang_pspec) (t:Type) = 
+  { wt : witnessable t }
 
-unfold
-let elab_typ0 (t:typ0) : Type u#0 = 
-  to_Type (to_shareable_typ t)
+instance targetlang_unit pspec : targetlang pspec unit = { wt = witnessable_unit }
+instance targetlang_int  pspec : targetlang pspec int = { wt = witnessable_int }
+instance targetlang_pair pspec t1 t2 {| c1:targetlang pspec t1 |} {| c2:targetlang pspec t2 |} 
+  : targetlang pspec (t1 * t2)
+  = { wt = witnessable_pair t1 t2 #c1.wt #c2.wt }
+instance targetlang_univ_raise pspec (t1:Type u#a) {| c1:targetlang pspec t1 |} 
+  : targetlang pspec (FStar.Universe.raise_t u#a u#b t1)
+  = { wt = witnessable_univ_raise t1 #c1.wt }
+instance targetlang_sum pspec t1 t2 {| c1:targetlang pspec t1 |} {| c2:targetlang pspec t2 |} 
+  : targetlang pspec (either t1 t2)
+  = { wt = witnessable_sum t1 t2 #c1.wt #c2.wt }
+instance targetlang_ref pspec t1 {| c1:targetlang pspec t1 |} 
+  : targetlang pspec (ref t1)
+  = { wt = witnessable_ref t1 #c1.wt }
+instance targetlang_llist pspec t1 {| c1:targetlang pspec t1 |} 
+  : targetlang pspec (linkedList t1)
+  = { wt = witnessable_llist t1 #c1.wt }
 
-let rec elab_typ0_tc (t:typ0) : witnessable (elab_typ0 t) = 
-  match t with
-  | TUnit -> witnessable_unit
-  | TNat -> witnessable_int
-  | TSum t1 t2 -> witnessable_sum _ _ #(elab_typ0_tc t1) #(elab_typ0_tc t2)
-  | TPair t1 t2 -> witnessable_pair _ _ #(elab_typ0_tc t1) #(elab_typ0_tc t2)
-  | TRef t -> witnessable_ref _ #(elab_typ0_tc t) 
-  | TLList t -> witnessable_llist _ #(elab_typ0_tc t)
-
-unfold let pre_tgt_arrow
+unfold let pre_targetlang_arrow
+  (inv:heap -> Type0)
+  (prref:ref_pred)
   (#t1:Type) {| c1 : witnessable t1 |}
-  (x:t1) =
-  sst_pre (fun h0 ->
-    c1.satisfy x h0 contains_pred /\
-    c1.satisfy x h0 is_shared)
+  (x:t1) (h0:heap) =
+  inv h0 /\ c1.satisfy x prref
 
-unfold let post_tgt_arrow
+unfold let post_targetlang_arrow
+  (inv:heap -> Type0)
+  (prref:ref_pred)
+  (hrel:FStar.Preorder.preorder heap)
   (#t1:Type) {| c1 : witnessable t1 |}
   (#t2:Type) {| c2 : witnessable t2 |}
-  (x:t1) =
-  sst_post t2 (pre_tgt_arrow #t1 #c1 x) (fun h0 r h1 -> 
-    gets_shared Set.empty h0 h1 /\
-    modifies_only_shared h0 h1 /\     (* allows shared references to be modified and to alloc new reference and share them *)
-    c2.satisfy r h1 contains_pred /\
-    c2.satisfy r h1 is_shared)
+  (x:t1) (h0:heap) (r:t2) (h1:heap) =
+  inv h1 /\ h0 `hrel` h1 /\ c2.satisfy r prref
 
-let mk_tgt_arrow
+let mk_targetlang_arrow
+  (pspec:targetlang_pspec)
   (t1:Type) {| c1 : witnessable t1 |}
   (t2:Type) {| c2 : witnessable t2 |}
 = x:t1 -> ST t2 
-    (requires (pre_tgt_arrow #t1 #c1 x ))
-    (ensures (post_tgt_arrow #t1 #c1 #t2 #c2 x))
+    (requires (fun h0 -> (Mktuple3?._1 pspec) h0 /\ c1.satisfy x (Mktuple3?._2 pspec))) (** CA: super stupid that one has to use projectors **)
+    (ensures (fun h0 r h1 -> (Mktuple3?._1 pspec) h1 /\ h0 `(Mktuple3?._3 pspec)` h1 /\ c2.satisfy r (Mktuple3?._2 pspec)))
 
-let rec lemma_123 (#t:typ0) (v:elab_typ0 t) h pred :
-  Lemma ((elab_typ0_tc t).satisfy v h pred <==> forall_refs_heap pred h #(to_shareable_typ t) v) 
-  // [SMTPat ((elab_typ0_tc t).satisfy v h pred); SMTPat (forallRefsHeap pred h #(to_shareable_typ t) v)]
-  by (compute ()) =
-  match t with
-  | TUnit -> ()
-  | TNat -> ()
-  | TSum t1 t2 -> begin
-    let v : either (elab_typ0 t1) (elab_typ0 t2) = v in
-    match v with
-    | Inl lv -> lemma_123 lv h pred
-    | Inr rv -> lemma_123 rv h pred
-  end
-  | TPair t1 t2 -> begin
-     let v : (elab_typ0 t1) * (elab_typ0 t2) = v in
-     lemma_123 (fst v) h pred;
-     lemma_123 (snd v) h pred;
-     assert ((elab_typ0_tc t).satisfy v h pred <==> forall_refs_heap pred h #(to_shareable_typ t) v)
-  end
-  | TRef t' -> 
-    let aux (#t':typ0) (v:elab_typ0 (TRef t')) : ref (elab_typ0 t') = v in
-    let v : ref (elab_typ0 t') = aux v in
-    assert ((elab_typ0_tc t).satisfy v h pred <==> forall_refs_heap pred h #(to_shareable_typ t) v) by (compute ())
-  | TLList t' -> begin
-    let aux (#t':typ0) (v:elab_typ0 (TLList t')) : linkedList (elab_typ0 t') = v in
-    let v : linkedList (elab_typ0 t') = aux v in
-    match v with
-    | LLNil -> ()
-    | LLCons v' xsref -> (
-      lemma_123 v' h pred;
-      let xsref : ref (linkedList (elab_typ0 t')) = xsref in
-      assert ((elab_typ0_tc t).satisfy v h pred <==> forall_refs_heap pred h #(to_shareable_typ t) v))
-  end
-
-open FStar.Universe
-
-let rec _elab_typ (t:typ) : tt:Type u#1 & witnessable tt =
-  match t with
-  | TArr t1 t2 -> begin
-    let tt1 = _elab_typ t1 in
-    let tt2 = _elab_typ t2 in
-    (| mk_tgt_arrow (dfst tt1) #(dsnd tt1) (dfst tt2) #(dsnd tt2),
-       witnessable_arrow (dfst tt1) (dfst tt2) (pre_tgt_arrow) (post_tgt_arrow)
-    |)
-  end 
-  | TUnit -> (| raise_t unit, solve |)
-  | TNat -> (| raise_t int, solve |)
-  | TSum t1 t2 ->
-    let (| tt1, c_tt1 |) = _elab_typ t1 in
-    let (| tt2, c_tt2 |) = _elab_typ t2 in
-    (| either tt1 tt2, witnessable_sum tt1 tt2 #c_tt1 #c_tt2 |)
-  | TPair t1 t2 ->
-    let (| tt1, c_tt1 |) = _elab_typ t1 in
-    let (| tt2, c_tt2 |) = _elab_typ t2 in
-    (| tt1 * tt2, witnessable_pair tt1 tt2 #c_tt1 #c_tt2 |)
-  | TRef _ ->
-    let tt = elab_typ0 t in
-    let c_tt = elab_typ0_tc t in
-    (| raise_t tt, witnessable_univ_raise _ #c_tt |)
-  | TLList t ->
-    let tt = elab_typ0 t in
-    let c_tt = elab_typ0_tc t in
-    (| raise_t (linkedList tt), witnessable_univ_raise _ #(witnessable_llist tt #c_tt) |)
-
-let elab_typ (t:typ) : Type =
-  dfst (_elab_typ t)
-
-let elab_typ_tc (t:typ) : witnessable (elab_typ t) =
-  dsnd (_elab_typ t)
-
-(** ** Examples **) 
-
-val ctx_update_ref_test : 
-  elab_typ (TArr (TRef TNat) TUnit)
-let ctx_update_ref_test y =
-  let y : ref int = downgrade_val y in
-  sst_write y (sst_read y + 1);
-  raise_val ()
-
-val ctx_update_multiple_refs_test : 
-  elab_typ (TArr (TRef (TRef TNat)) (TArr (TRef TNat) TUnit))
-let ctx_update_multiple_refs_test x =
-  let x : ref (ref int) = downgrade_val x in
-  witness (contains_pred x);
-  witness (is_shared x);
-  let cb : elab_typ (TArr (TRef TNat) TUnit) = (fun y ->
-    let y : ref int = downgrade_val y in
-    recall (contains_pred x);
-    let ix : ref int = sst_read #(SRef SNat) x in
-    recall (is_shared x);   
-    sst_write #SNat ix (sst_read ix + 1);
-    sst_write #(SRef SNat) x y;
-    sst_write #SNat y (sst_read y + 5);
-    raise_val () 
-  ) in
-  cb
-
-val ctx_HO_test1 : 
-  elab_typ (TArr (TRef (TPair (TRef TNat) (TRef TNat))) (TArr TUnit TUnit))
-let ctx_HO_test1 xs =
-  let h0 = get () in
-  let xs : ref ((ref int) * ref int) = downgrade_val xs in
-  let (x', x'') : (ref int) * ref int = sst_read #(SPair (SRef SNat) (SRef SNat)) xs in
-  sst_write #(SPair (SRef SNat) (SRef SNat)) xs (x', x');
-  witness (contains_pred xs); witness (contains_pred x'); witness (contains_pred x'');
-  witness (is_shared xs); witness (is_shared x'); witness (is_shared x'');
-  (fun _ -> 
-    recall (contains_pred xs); recall (contains_pred x'); recall (contains_pred x'');
-    recall (is_shared xs); recall (is_shared x'); recall (is_shared x'');
-    sst_write #(SPair (SRef SNat) (SRef SNat)) xs (x', x'');
-    raise_val ())
-  
-val ctx_identity :
-  elab_typ (TArr (TRef TNat) (TRef TNat))
-let ctx_identity x = x
-
-val ctx_HO_test2 :
-  elab_typ (TArr (TArr TUnit (TRef TNat)) TUnit)
-let ctx_HO_test2 f =
-  let x:ref int = downgrade_val (f (raise_val ())) in
-  sst_write #SNat x (!x + 1);
-  raise_val ()
-
-val ctx_swap_ref_test :
-  elab_typ (TArr (TRef (TRef TNat)) (TArr (TRef (TRef TNat)) TUnit))
-let ctx_swap_ref_test x =
-  let x : ref (ref int) = downgrade_val x in
-  witness (contains_pred x);
-  witness (is_shared x);
-  let cb : elab_typ (TArr (TRef (TRef TNat)) TUnit) = (fun y ->
-    let y : ref (ref int) = downgrade_val y in
-    recall (contains_pred x);
-    recall (is_shared x);
-    
-    let z = sst_read x in
-    let t = sst_read y in
-    sst_write #(SRef SNat) x t;
-    sst_write #(SRef SNat) y z;
-
-    raise_val ()) in
-  cb
-
-val ctx_dynamic_alloc_test :
-   elab_typ (TArr TUnit (TRef TNat))
-let ctx_dynamic_alloc_test _ = 
-  let v = sst_alloc_shared #SNat 0 in 
-  raise_val v
-
-val ctx_HO_test3 :
-  elab_typ (TArr (TArr TUnit (TRef TNat)) TUnit)
-let ctx_HO_test3 f =
-  let x:ref int = downgrade_val (f (raise_val ())) in
-  let y:ref int = sst_alloc_shared #SNat (!x + 1) in
-  raise_val ()
-
-#push-options "--split_queries always"
-val ctx_returns_callback_test :
-  elab_typ (TArr TUnit (TArr TUnit TUnit))
-let ctx_returns_callback_test _ =
-  let x: ref int = sst_alloc_shared #SNat 13 in
-  witness (contains_pred x);
-  witness (is_shared x);
-  let cb : elab_typ (TArr TUnit TUnit) = (fun _ ->
-    recall (contains_pred x);
-    recall (is_shared x);
-    sst_write #SNat x (sst_read x % 5);
-    raise_val ()
-  ) in
-  cb
-#pop-options
-
-val ctx_HO_test4 :
-  elab_typ (TArr (TArr TUnit (TRef TNat)) TUnit)
-let ctx_HO_test4 f =
-  let x:ref int = downgrade_val (f (raise_val ())) in
-  let y:ref (ref int) = sst_alloc_shared #(SRef SNat) x in
-  raise_val ()
-
-val progr_sep_test: 
-  #rp: ref int -> 
-  ctx:(elab_typ (TArr TUnit TUnit)) ->
-  SST unit
-    (requires (fun h0 -> 
-      satisfy rp h0 contains_pred /\
-      ~(is_shared rp h0)))
-    (ensures (fun h0 _ h1 ->
-      sel h0 rp == sel h1 rp)) // the content of rp should stay the same before/ after calling the context
-         
-let progr_sep_test #rp f = (** If this test fails, it means that the spec of f does not give [automatically] separation  **)
-  downgrade_val (f (raise_val ()))
-
-val progr_declassify :
-  rp: ref int -> 
-  ctx:(elab_typ (TArr (TRef TNat) TUnit)) ->
-  SST unit
-    (requires (fun h0 -> 
-      satisfy rp h0 contains_pred /\
-      ~(is_shared rp h0)))
-    (ensures (fun h0 _ h1 -> True))
-let progr_declassify rp f =
-  let h0 = get () in
-  sst_share #SNat rp;
-  let h1 = get () in
-  let r = downgrade_val (f (raise_val rp)) in  
-  r
-
-val progr_declassify_nested:
-  rp: ref (ref int) -> 
-  ctx:(elab_typ (TArr (TRef (TRef TNat)) TUnit)) ->
-  SST unit
-    (requires (fun h0 -> 
-      satisfy rp h0 contains_pred /\
-      ~(is_shared rp h0)))
-    (ensures (fun h0 _ h1 -> True))
-let progr_declassify_nested rp f =
-  let p : ref int = sst_read #(SRef SNat) rp in
-  sst_share #SNat p;
-  sst_share #(SRef SNat) rp;
-  // let r = elab_alloc (!rp) in (* <-- needed a copy here! *) 
-  downgrade_val (f (raise_val rp))
-
-val progr_secret_unchanged_test: 
-  rp: ref int -> 
-  rs: ref (ref int) ->
-  ctx:(elab_typ (TArr TUnit TUnit)) ->
-  SST unit 
-    (requires (fun h0 -> 
-      satisfy rp h0 contains_pred /\
-      ~(is_shared rp h0) /\
-      satisfy rs h0 is_shared))
-    (ensures (fun h0 _ h1 ->
-      sel h0 rp == sel h1 rp))
-         
-let progr_secret_unchanged_test rp rs ctx = 
-  let h0 = get () in
-  let secret: ref int = sst_alloc #SNat 0 in
-  let h1 = get () in
-  downgrade_val (ctx (raise_val ()));
-  let v = sst_read #SNat secret in
-  ()
-
-val progr_passing_callback_test: 
-  rp: ref int -> 
-  rs: ref (ref int) ->
-  ctx:(elab_typ (TArr (TArr TUnit TUnit) TUnit)) ->
-  SST unit 
-    (requires (fun h0 ->
-      satisfy rp h0 contains_pred /\
-      ~(is_shared rp h0) /\
-      satisfy rs h0 is_shared))
-    (ensures (fun h0 _ h1 -> sel h0 rp == sel h1 rp)) // the content of rp should stay the same before/ after calling the context
-
-// TODO: the callback of the program should be able to modify rp
-let progr_passing_callback_test rp rs f =
-  let secret: ref int = sst_alloc #SNat 0 in
-  sst_share #SNat secret;
-  witness (contains_pred secret);
-  witness (is_shared secret);
-  let cb: elab_typ (TArr TUnit TUnit) = (fun _ -> 
-    recall (contains_pred secret);
-    recall (is_shared secret);
-    sst_write #SNat secret (!secret + 1);
-    raise_val ()) in
-  downgrade_val (f cb);
-  ()
-
-val progr_getting_callback_test: 
-  rp: ref int -> 
-  rs: ref (ref int) ->
-  ctx:(elab_typ (TArr TUnit (TArr TUnit TUnit))) ->
-  SST unit 
-    (requires (fun h0 ->
-      satisfy rp h0 contains_pred /\
-      ~(is_shared rp h0) /\
-      satisfy rs h0 is_shared))
-    (ensures (fun h0 _ h1 -> sel h0 rp == sel h1 rp))
-let progr_getting_callback_test rp rs f =
-  let cb = f (raise_val ()) in
-  downgrade_val (cb (raise_val ()));
-  ()
+instance targetlang_arrow pspec t1 t2 {| c1:targetlang pspec t1 |} {| c2:targetlang pspec t2 |}
+  : targetlang pspec (mk_targetlang_arrow pspec t1 #c1.wt t2 #c2.wt)
+  = { wt = witnessable_arrow t1 t2 _ _ }
