state/Witnessable.fst
@@ -12,33 +12,37 @@ type ref_lheap_pred =
   pred:(#a:Type -> #rel:_ -> mref a rel -> heap -> Type0){forall (a:Type) (x:ref a) h0 h1. pred x h0 /\ h0 `heap_rel` h1 ==> pred x h1}
 
 class witnessable (t:Type) = {
-  satisfy : t -> heap -> ref_lheap_pred -> Type0;
+  satisfy : t -> (#a:_ -> #rel:_ -> mref a rel -> Type0) -> Type0;
+  satisfy_on_heap : t -> heap -> ref_lheap_pred -> Type0;
 
-  satisfy_monotonic : x:t -> pred:ref_lheap_pred -> h0:heap -> h1:heap -> Lemma (
-    h0 `heap_rel` h1 /\ satisfy x h0 pred ==> satisfy x h1 pred);
+  satisfy_on_heap_monotonic : x:t -> pred:ref_lheap_pred -> h0:heap -> h1:heap -> Lemma (
+    h0 `heap_rel` h1 /\ satisfy_on_heap x h0 pred ==> satisfy_on_heap x h1 pred);
 
-  pwitness : x:t -> pred:ref_lheap_pred -> ST (precall:(unit -> ST unit (fun _ -> True) (fun h0 _ h1 -> h0 == h1 /\ satisfy x h1 pred)))
-    (requires (fun h0 -> satisfy x h0 pred))
+  pwitness : x:t -> pred:ref_lheap_pred -> ST (precall:(unit -> ST unit (fun _ -> True) (fun h0 _ h1 -> h0 == h1 /\ satisfy_on_heap x h1 pred)))
+    (requires (fun h0 -> satisfy_on_heap x h0 pred))
     (ensures (fun h0 _ h1 -> h0 == h1));
 }
 
 instance witnessable_ref (t:Type) {| c:witnessable t |} : witnessable (ref t) = {
-  satisfy = (fun x h pred -> pred x h);
-  satisfy_monotonic = (fun x pred h0 h1 -> ());
+  satisfy = (fun x pred -> pred x);
+  satisfy_on_heap = (fun x h pred -> pred x h);
+  satisfy_on_heap_monotonic = (fun x pred h0 h1 -> ());
   pwitness = (fun x pred ->
     MST.Tot.witness (pred x);
     (fun () -> MST.Tot.recall (pred x)))
 }
 
 instance witnessable_unit : witnessable unit = {
-  satisfy = (fun _ _ _ -> True);
-  satisfy_monotonic = (fun _ _ _ _ -> ());
+  satisfy = (fun _ _ -> True);
+  satisfy_on_heap = (fun _ _ _ -> True);
+  satisfy_on_heap_monotonic = (fun _ _ _ _ -> ());
   pwitness = (fun _ _ -> (fun () -> ()));
 }
 
 instance witnessable_int : witnessable int = {
-  satisfy = (fun _ _ _ -> True);
-  satisfy_monotonic = (fun _ _ _ _ -> ());
+  satisfy = (fun _ _ -> True);
+  satisfy_on_heap = (fun _ _ _ -> True);
+  satisfy_on_heap_monotonic = (fun _ _ _ _ -> ());
   pwitness = (fun _ _ -> (fun () -> ()));
 }
 
@@ -47,16 +51,18 @@ instance witnessable_arrow
   (pre:t1 -> st_pre)
   (post:(x:t1 -> h0:heap -> st_post' t2 (pre x h0))) // TODO: one cannot have pre-post depending on outside things.
 : witnessable (x:t1 -> ST t2 (pre x) (post x)) = {
-  satisfy = (fun _ _ _ -> True);
-  satisfy_monotonic = (fun _ _ _ _ -> ());
+  satisfy = (fun _ _ -> True);
+  satisfy_on_heap = (fun _ _ _ -> True);
+  satisfy_on_heap_monotonic = (fun _ _ _ _ -> ());
   pwitness = (fun _ _ -> (fun () -> ()));
 }
 
 instance witnessable_pair (t1:Type) (t2:Type) {| c1:witnessable t1 |} {| c2:witnessable t2 |} : witnessable (t1 * t2) = {
-  satisfy = (fun (x1, x2) h pred -> c1.satisfy x1 h pred /\ c2.satisfy x2 h pred);
-  satisfy_monotonic = (fun (x1, x2) pred h0 h1 -> 
-    c1.satisfy_monotonic x1 pred h0 h1;
-    c2.satisfy_monotonic x2 pred h0 h1);
+  satisfy = (fun (x1, x2) pred -> c1.satisfy x1 pred /\ c2.satisfy x2 pred);
+  satisfy_on_heap = (fun (x1, x2) h pred -> c1.satisfy_on_heap x1 h pred /\ c2.satisfy_on_heap x2 h pred);
+  satisfy_on_heap_monotonic = (fun (x1, x2) pred h0 h1 -> 
+    c1.satisfy_on_heap_monotonic x1 pred h0 h1;
+    c2.satisfy_on_heap_monotonic x2 pred h0 h1);
   pwitness = (fun (x1, x2) pred -> 
     let w1 = c1.pwitness x1 pred in
     let w2 = c2.pwitness x2 pred in
@@ -64,14 +70,18 @@ instance witnessable_pair (t1:Type) (t2:Type) {| c1:witnessable t1 |} {| c2:witn
 }
 
 instance witnessable_sum (t1:Type) (t2:Type) {| c1:witnessable t1 |} {| c2:witnessable t2 |} : witnessable (either t1 t2) = {
-  satisfy = (fun x h pred ->
+  satisfy = (fun x pred ->
     match x with
-    | Inl x1 -> c1.satisfy x1 h pred
-    | Inr x2 -> c2.satisfy x2 h pred);
-  satisfy_monotonic = (fun x pred h0 h1 ->
+    | Inl x1 -> c1.satisfy x1 pred
+    | Inr x2 -> c2.satisfy x2 pred);
+  satisfy_on_heap = (fun x h pred ->
     match x with
-    | Inl x1 -> c1.satisfy_monotonic x1 pred h0 h1
-    | Inr x2 -> c2.satisfy_monotonic x2 pred h0 h1);
+    | Inl x1 -> c1.satisfy_on_heap x1 h pred
+    | Inr x2 -> c2.satisfy_on_heap x2 h pred);
+  satisfy_on_heap_monotonic = (fun x pred h0 h1 ->
+    match x with
+    | Inl x1 -> c1.satisfy_on_heap_monotonic x1 pred h0 h1
+    | Inr x2 -> c2.satisfy_on_heap_monotonic x2 pred h0 h1);
   pwitness = (fun x pred -> 
     match x with 
     | Inl x1 -> (let w = c1.pwitness x1 pred in (fun () -> w ()))
@@ -79,16 +89,20 @@ instance witnessable_sum (t1:Type) (t2:Type) {| c1:witnessable t1 |} {| c2:witne
 }
 
 instance witnessable_llist (t:Type) {| c:witnessable t |} : witnessable (linkedList t) = {
-  satisfy = (fun l h pred -> 
+  satisfy = (fun l pred ->
     match l with
     | LLNil -> True
-    | LLCons x xsref -> c.satisfy x h pred /\ pred xsref h
+    | LLCons x xsref -> c.satisfy x pred /\ pred xsref);
+  satisfy_on_heap = (fun l h pred -> 
+    match l with
+    | LLNil -> True
+    | LLCons x xsref -> c.satisfy_on_heap x h pred /\ pred xsref h
   );
 
-  satisfy_monotonic = (fun l pred h0 h1 ->
+  satisfy_on_heap_monotonic = (fun l pred h0 h1 ->
     match l with 
     | LLNil -> ()
-    | LLCons x xsref -> c.satisfy_monotonic x pred h0 h1
+    | LLCons x xsref -> c.satisfy_on_heap_monotonic x pred h0 h1
   );
 
   pwitness = (fun l pred ->
@@ -103,6 +117,7 @@ instance witnessable_llist (t:Type) {| c:witnessable t |} : witnessable (linkedL
 
 instance witnessable_univ_raise (t:Type u#a) {| c:witnessable t |} : witnessable (raise_t u#a u#b t) = {
   satisfy = (fun x -> c.satisfy (downgrade_val x));
-  satisfy_monotonic = (fun x -> c.satisfy_monotonic (downgrade_val x));
+  satisfy_on_heap = (fun x -> c.satisfy_on_heap (downgrade_val x));
+  satisfy_on_heap_monotonic = (fun x -> c.satisfy_on_heap_monotonic (downgrade_val x));
   pwitness = (fun x -> c.pwitness (downgrade_val x));
 }
